kuiops/sdpa/Kuiops.Sdpa.Flash.Kf.fsti
@@ -20,6 +20,7 @@ open Kuiper.EMatrix
 open Kuiper.ForEvery
 open Kuiper.Shape
 open Pulse.Lib.Pledge
+open Kuiops.Sdpa.Flash.Vals
 open Kuiops.Sdpa.Flash.Types
 
 module SZ = Kuiper.SizeT
@@ -105,7 +106,14 @@ fn sdpa_flash_kf
          (SZ.v bi) (SZ.v kvh) (SZ.v group) (SZ.v r0))
       (flash_eL_at nw d b hq sq rows sk eQ eKg emask has_mask causal scale
          (SZ.v bi) (SZ.v kvh) (SZ.v group) (SZ.v r0))
-      shscale shO shgm shgl tid bi r0 group kvh
+      shscale shO shgm shgl
+      (flash_escale_at nw d b hq sq rows sk eQ eKg emask has_mask causal scale
+         (SZ.v bi) (SZ.v kvh) (SZ.v group) (SZ.v r0))
+      (flash_eO_at nw d b hq sq rows sk eQ eKg eVg emask has_mask causal scale
+         (SZ.v bi) (SZ.v kvh) (SZ.v group) (SZ.v r0))
+      (flash_egl_at nw d b hq sq rows sk eQ eKg emask has_mask causal scale
+         (SZ.v bi) (SZ.v kvh) (SZ.v group) (SZ.v r0))
+      tid bi r0 group kvh
       #fQ #fKg #fVg #fmask #eQ #eKg #eVg #emask
   ensures
     sdpa_flash_post #et_ab #et_acc nw nthr d sk b hq sq rows
@@ -116,7 +124,14 @@ fn sdpa_flash_kf
          (SZ.v bi) (SZ.v kvh) (SZ.v group) (SZ.v r0))
       (flash_eL_at nw d b hq sq rows sk eQ eKg emask has_mask causal scale
          (SZ.v bi) (SZ.v kvh) (SZ.v group) (SZ.v r0))
-      shscale shO shgl tid bi r0 group kvh
+      shscale shO shgl
+      (flash_escale_at nw d b hq sq rows sk eQ eKg emask has_mask causal scale
+         (SZ.v bi) (SZ.v kvh) (SZ.v group) (SZ.v r0))
+      (flash_eO_at nw d b hq sq rows sk eQ eKg eVg emask has_mask causal scale
+         (SZ.v bi) (SZ.v kvh) (SZ.v group) (SZ.v r0))
+      (flash_egl_at nw d b hq sq rows sk eQ eKg emask has_mask causal scale
+         (SZ.v bi) (SZ.v kvh) (SZ.v group) (SZ.v r0))
+      tid bi r0 group kvh
       #fQ #fKg #fVg #fmask #eQ #eKg #eVg #emask **
     if_ (combine_active 16sz
       (sdpa_flash_w nw nthr tid) (sdpa_flash_lane nw nthr tid))
